Alternative encryption without an accumulator (makes induction proofs much simpler), and the proofof enc_loop m = enc_loop c

BG_formalization.thy
@@ -44,13 +44,29 @@ text "We define the loop in the encryption as a recursive function. This functio
 fun enc_loop_func 
   :: "((nat  => bitstring) \<times> nat \<times> nat \<times> bitstring list) \<Rightarrow> bitstring list \<Rightarrow> nat \<Rightarrow> (bitstring list \<times> nat)" 
   where
-   "enc_loop_func (f, n, h, []) c_acc x = (c_acc, x)" |
+   "enc_loop_func (f, n, h, []) c_acc x = (rev c_acc, x)" |
    "enc_loop_func (f, n, h, (m_i # m_rest)) c_acc x =
         (let x_i = x * x mod n in
         let p_i = f (x_i mod 2^h) in
         let c_i = m_i [\<oplus>] p_i in
         enc_loop_func (f, n, h, m_rest) (c_i # c_acc) x_i
         )"
+
+fun enc_loop_func_list 
+  :: "((nat  => bitstring) \<times> nat \<times> nat \<times> bitstring list) \<Rightarrow> nat \<Rightarrow> bitstring list" 
+  where
+   "enc_loop_func_list (f, n, h, []) x = []" |
+   "enc_loop_func_list (f, n, h, (m_i # m_rest)) x =
+        (let x_i = x * x mod n in
+        let p_i = f (x_i mod 2^h) in
+        let c_i = m_i [\<oplus>] p_i in
+        c_i # enc_loop_func_list (f, n, h, m_rest) x_i
+        )"
+fun enc_loop_func_x 
+  :: "((nat  => bitstring) \<times> nat \<times> nat \<times> nat) \<Rightarrow> nat \<Rightarrow> nat" 
+  where
+   "enc_loop_func_x (f, n, h, t) x = x ^ (2 ^ t) mod n" 
+
 
 
 text "A simple function to convert a bit represented by a natural number to a bit represented by a 
@@ -60,6 +76,8 @@ fun nat_to_bit :: "nat \<Rightarrow> bool" where
   case_0: "nat_to_bit 0 = False" | 
   case_1: "nat_to_bit (Suc 0) = True" |
   case_greater: "nat_to_bit (Suc (Suc n)) = False"
+
+
 
 
 text "The function gives False for anything other than True."
@@ -76,6 +94,14 @@ fun enc_loop
    "enc_loop (n, h, m) x 
     = enc_loop_func (nat_to_bitstring h, n, h, m) [] x"
 
+fun enc_loop_alt 
+   :: "(nat \<times> nat \<times> bitstring list) \<Rightarrow> nat \<Rightarrow> (bitstring list \<times> nat)" 
+   where
+   "enc_loop_alt (n, h, m) x 
+    = (enc_loop_func_list (nat_to_bitstring h, n, h, m) x, 
+      enc_loop_func_x (nat_to_bitstring h, n, h, length m) x)"
+
+
 text "At last, the encryption function:"
 definition encrypt :: "nat \<Rightarrow> bitstring \<Rightarrow> nat \<Rightarrow> (bitstring list \<times> nat)" where
   "encrypt n m r = (
@@ -85,6 +111,20 @@ definition encrypt :: "nat \<Rightarrow> bitstring \<Rightarrow> nat \<Rightarro
   let (c, x_t) = enc_loop (n, h, m_l) x_0 in 
   let x_t' = x_t * x_t mod n in 
   (c, x_t'))"
+
+definition encrypt_alt :: "nat \<Rightarrow> bitstring \<Rightarrow> nat \<Rightarrow> (bitstring list \<times> nat)" where
+  "encrypt_alt n m r = (
+  let h = nat \<lfloor>log 2 (log 2 n)\<rfloor> in 
+  let m_l = split m h in 
+  let (x_0 :: nat) = (r * r) mod n in 
+  let (c, x_t) = enc_loop_alt (n, h, m_l) x_0 in 
+  let x_t' = x_t * x_t mod n in 
+  (c, x_t'))"
+
+
+
+
+
 
 
 text "An alternate definition of floor log:"
@@ -110,6 +150,12 @@ definition encrypt_discrete_log :: "nat \<Rightarrow> bitstring \<Rightarrow> na
   (c, x_t'))"
 
 
+
+
+
+
+
+
 text "now the decryption..."
 
 fun calculate_exponent :: "nat \<Rightarrow> nat \<Rightarrow> nat" where 
@@ -129,16 +175,35 @@ definition decrypt :: "nat \<Rightarrow> nat \<Rightarrow> (bitstring list \<tim
     let (m, x') = enc_loop (p * q, (nat \<lfloor>log 2 (log 2 (p * q))\<rfloor>) , c) x_0 in
     merge_list m))"
 
+definition decrypt_alt :: "nat \<Rightarrow> nat \<Rightarrow> (bitstring list \<times> nat) \<Rightarrow> bitstring" where
+  "decrypt_alt p q tup = (case tup of (c, x) \<Rightarrow> 
+   (let u_p = x ^ (calculate_exponent (length c) p) in
+    let u_q = x ^ (calculate_exponent (length c) q) in
+    let ((r_p, r_q), _) = euclid_ext p q in
+    let x_0 = nat (u_p * r_p * p + u_q * r_q * q mod (p * q)) in
+    let (m, x') = enc_loop_alt (p * q, (nat \<lfloor>log 2 (log 2 (p * q))\<rfloor>) , c) x_0 in
+    merge_list m))"
+
+
+
+
+
+
+
+
+
+
+
 text "Correctness proof"
 
 lemma enc_loop_func_exp: 
-  assumes "n > 0" "h > 0" "x < n"
+  assumes "n > 0" "x < n"
   shows "snd (enc_loop_func (nat_to_bitstring h, n, h, m) c x) = x ^ (2 ^ (length m)) mod n"
   using assms
 proof (induction m arbitrary: x c)
   case Nil
-  then have "(enc_loop_func (nat_to_bitstring h, n, h, []) c x) = (c, x)" using enc_loop_func.simps(1) by auto
-  then show ?case using local.Nil(3) by auto
+  then have "(enc_loop_func (nat_to_bitstring h, n, h, []) c x) = (rev c, x)" using enc_loop_func.simps(1) by auto
+  then show ?case using local.Nil(2) by auto
 next
   case (Cons a m)
   then have enc_loop_def: "snd (enc_loop_func (nat_to_bitstring h, n, h, (a # m)) c x) = snd(
@@ -163,10 +228,88 @@ next
   from this x_times_x show ?case by auto
 qed
 
+corollary enc_loop_x: 
+  assumes "n > 0" "x < n"
+  shows "snd (enc_loop_func (nat_to_bitstring h, n, h, m) c x) = snd (enc_loop_alt (n, h, m) x)"
+  by (auto intro: enc_loop_func_exp simp add: assms)
+
+corollary enc_loop_x_enc_loop_normal: 
+  assumes "n > 0" "x < n"
+  shows "snd (enc_loop (n, h, m) x) = snd (enc_loop_alt (n, h, m) x)"
+  by (auto intro: enc_loop_func_exp simp add: assms)
+
 corollary enc_loop_exp: 
   assumes "n > 0" "h > 0" "x < n"
   shows "snd (enc_loop (n, h, m) x) = x ^ (2 ^ (length m)) mod n"
   by (auto intro: enc_loop_func_exp simp add: assms)
+
+theorem enc_x_exp: 
+  assumes "n > 0" "r < n" "h = nat \<lfloor>log 2 (log 2 n)\<rfloor>" "m_l = split m h"
+  shows "snd (encrypt n m r) = (r * r) ^ (2 ^ (length m_l + 1)) mod n"
+proof - 
+  from encrypt_def have encrypt_open: "snd (encrypt n m r) = snd (
+  let h = nat \<lfloor>log 2 (log 2 n)\<rfloor> in 
+  let m_l = split m h in 
+  let (x_0 :: nat) = (r * r) mod n in 
+  let (c, x_t) = enc_loop (n, h, m_l) x_0 in 
+  let x_t' = x_t * x_t mod n in 
+  (c, x_t'))" by auto
+  
+  have "r * r mod n < n" using mod_less_divisor assms(1) by auto
+
+  then have  "snd (
+  let h = nat \<lfloor>log 2 (log 2 n)\<rfloor> in 
+  let m_l = split m h in 
+  let (x_0 :: nat) = (r * r) mod n in 
+  enc_loop (n, h, m_l) x_0) = 
+  (let h = nat \<lfloor>log 2 (log 2 n)\<rfloor> in 
+  let m_l = split m h in 
+  let (x_0 :: nat) = (r * r) mod n in 
+  (x_0 ^ (2 ^ (length m_l)) mod n))" using assms(1) enc_loop.simps enc_loop_func_exp
+    by (metis)
+  from encrypt_open this have "snd (
+  let h = nat \<lfloor>log 2 (log 2 n)\<rfloor> in 
+  let m_l = split m h in 
+  let (x_0 :: nat) = (r * r) mod n in 
+  let (c, x_t) = enc_loop (n, h, m_l) x_0 in 
+  let x_t' = x_t * x_t mod n in 
+  (c, x_t'))
+  = 
+  (let h = nat \<lfloor>log 2 (log 2 n)\<rfloor> in 
+  let m_l = split m h in 
+  let (x_0 :: nat) = (r * r) mod n in 
+  let x_t' = x_0 ^ (2 ^ (length m_l)) mod n in 
+  x_t' * x_t' mod n)" 
+  using old.prod.exhaust snd_conv split_conv
+  by (smt (verit, best)) 
+
+  then have  "snd (
+  let h = nat \<lfloor>log 2 (log 2 n)\<rfloor> in 
+  let m_l = split m h in 
+  let (x_0 :: nat) = (r * r) mod n in 
+  let (c, x_t) = enc_loop (n, h, m_l) x_0 in 
+  let x_t' = x_t * x_t mod n in 
+  (c, x_t'))
+  = 
+  (((r * r) mod n) ^ (2 ^ (length m_l)) mod n) * (((r * r) mod n) ^ (2 ^ (length m_l)) mod n) mod n" 
+  using assms 
+  by meson
+
+  then have "snd (encrypt n m r) = (((r * r) mod n) ^ (2 ^ (length m_l)) mod n) * (((r * r) mod n) ^ (2 ^ (length m_l)) mod n) mod n" 
+    using encrypt_open by auto
+  then have "snd (encrypt n m r) = ((r * r) ^ (2 ^ (length m_l)) mod n) * ((r * r) ^ (2 ^ (length m_l)) mod n) mod n"
+    using power_mod by metis
+  then have encrypt_to_exp: "snd (encrypt n m r) = (((r * r) ^ (2 ^ (length m_l))) * ((r * r) ^ (2 ^ (length m_l)))) mod n"
+    by (simp add: mod_mult_eq) 
+
+  have "(((r * r) ^ (2 ^ (length m_l))) * ((r * r) ^ (2 ^ (length m_l)))) = (r * r) ^ (2 ^ (length m_l) + 2 ^ (length m_l))" 
+    using power_add[symmetric] by auto
+  then have "(((r * r) ^ (2 ^ (length m_l))) * ((r * r) ^ (2 ^ (length m_l)))) = (r * r) ^ (2 * 2 ^ (length m_l))"
+    by (simp add: mult_2)
+  then have "(((r * r) ^ (2 ^ (length m_l))) * ((r * r) ^ (2 ^ (length m_l)))) = (r * r) ^ (2 ^ (length m_l + 1))"
+    by auto
+  from this encrypt_to_exp show ?thesis by auto
+qed
 
 
 lemma same_x_0:
@@ -184,6 +327,7 @@ proof -
 
   show ?thesis sorry
 qed 
+
 
 theorem 
   assumes 
@@ -207,56 +351,81 @@ proof -
     using prod.exhaust prod.sel(1) prod.simps(2)
     by (metis (mono_tags, lifting))
 
-
-  have "(let h = nat \<lfloor>log 2 (log 2 (real p * real q))\<rfloor> in nat_to_bitstring h) =
-     nat_to_bitstring (nat \<lfloor>log 2 (log 2 (real p * real q))\<rfloor>)" by auto
-  
+  have "\<exists>c x. (encrypt (p * q) m r = (c, x))" using encrypt_def surj_pair by 
+  by auto
+  then obtain c x where "(encrypt (p * q) m r = (c, x))" by blast
+  then have "decrypt p q (encrypt (p * q) m r) = decrypt p q (c, x)" by auto
+  hence "decrypt p q (encrypt (p * q) m r) =  
+   (let u_p = x ^ (calculate_exponent (length c) p) in
+    let u_q = x ^ (calculate_exponent (length c) q) in
+    let ((r_p, r_q), _) = euclid_ext p q in
+    let x_0 = nat (u_p * r_p * p + u_q * r_q * q mod (p * q)) in
+    let (m, x') = enc_loop (p * q, (nat \<lfloor>log 2 (log 2 (p * q))\<rfloor>) , c) x_0 in
+    merge_list m)" using decrypt_def by auto  
 
    show ?thesis sorry
-qed
+ qed
 
+ 
+lemma h_not_smaller: "h \<ge> length (nat_to_words (Suc 0) (p mod 2 ^ h))"
+  by (simp add: nat_bnd_word_len)
 
+lemma length_eq: "length (nat_to_bitstring h (p mod 2^h)) = h" 
+  by (auto simp add: nat_to_bitstring_def nat_to_words_len_def h_not_smaller) 
 
-text "This formalization, using logarithms makes our proofs harder by introducing real numbers. Now,
-we try to formalize the floor of a logarithm's logarithm without logarithms"
+text "Here, we show that if we find the x_0, then we can recover the plaintext message 
+    from encrypted message c."
 
-lemma
-  fixes n::nat
-  assumes "n \<ge> 1" "base > (Suc 0)" 
-  shows "floor_nat_log base n = \<lfloor>log base n\<rfloor>"
-  using assms(1)
-proof (induction n rule: dec_induct)
-    
-  case base \<comment> \<open>n = 1\<close>
+lemma enc_loop_alt_correctness:
+  assumes "x > 0" "n > 0" "h > 0" "x < n" 
+  shows  "\<lbrakk>\<forall>l \<in> set m. length l \<le> h; c = fst (enc_loop_alt (n, h, m) x)\<rbrakk> \<Longrightarrow> 
+          fst (enc_loop_alt (n, h, c) x) = m"
 
-  have "floor_nat_log base 1 = floor_nat_log_rec base (Suc 0) 0 "  
-    by (auto simp add: floor_nat_log_def )
-  then have "floor_nat_log base 1 
-    = floor_nat_log_rec base ((Suc 0) div base) (Suc 0)"
-    using Suc_less_eq2 floor_nat_log_rec.simps(5) gr0_implies_Suc assms(2)
-    by (metis)
-  also have "(Suc 0) div base = 0" 
-    by (simp add: assms(2)) 
-  moreover have "floor_nat_log base 1 
-    = floor_nat_log_rec base 0 (Suc 0)"
-      using calculation by simp
-  then have  "floor_nat_log base 1  = 0 "
-    using Nat.lessE assms(2) floor_nat_log_rec.simps(4) 
-    by (metis)
-  then show ?case by simp
+proof (induction m arbitrary: c x)
+  case Nil
+  then show ?case by auto
 next
-  case (step n)
-  have "\<lfloor>log base n\<rfloor> = \<lfloor>ln n / ln base\<rfloor>" by (auto simp add: log_def)
-  
-  
-  then show ?case sorry
+  let ?f = "nat_to_bitstring h"
+  case (Cons a m)
+  assume "\<forall>l \<in> set (a # m). length l \<le> h" 
+  assume "c = fst (enc_loop_alt (n, h, a # m) x)"
+
+  then have "c = enc_loop_func_list (?f, n, h, a # m) x" by auto
+  then have c_def: "c = (let x_i = x * x mod n in
+        let p_i = ?f (x_i mod 2^h) in
+        let c_i = a [\<oplus>] p_i in
+        c_i # enc_loop_func_list (nat_to_bitstring h, n, h, m) x_i
+        )" by auto
+  let ?a' = "(a [\<oplus>] ?f (x * x mod n mod 2^h))"
+
+  from c_def have c_part: "c = ?a' # enc_loop_func_list (nat_to_bitstring h, n, h, m) (x * x mod n)" by metis
+  then have "\<exists>c'. c = ?a' # c'" by auto
+  then obtain c' where c_obtain: "c = ?a' # c'" by blast
+  from this c_part have "c' = enc_loop_func_list (nat_to_bitstring h, n, h, m) (x * x mod n)" by auto
+  hence "fst (enc_loop_alt (n, h, c') (x * x mod n)) = m" using Cons by auto
+  hence a_with_m: "a # fst (enc_loop_alt (n, h, c') (x * x mod n)) = a # m" by auto
+
+   have a_xor_bot: "?a' [\<oplus>] ?f (x * x mod n mod 2^h) = a [\<oplus>] (replicate (length (?f (x * x mod n mod 2^h))) bot)"
+    by (auto simp add: xor_list_inverse)
+
+  have "length a \<le> h" using Cons(2) by auto
+  then have "a [\<oplus>] (replicate (length (?f (x * x mod n mod 2^h))) bot) = a" 
+    using xor_replicate_bot_right length_eq by auto 
+
+  from this a_xor_bot have "?a' [\<oplus>] ?f (x * x mod n mod 2^h) = a" by auto
+
+  from this a_with_m 
+  have "?a' [\<oplus>] ?f (x * x mod n mod 2^h) # fst (enc_loop_alt (n, h, c') (x * x mod n)) = a # m"
+    by auto
+
+  hence "(let x_i = x * x mod n in
+        let p_i = ?f (x_i mod 2^h) in
+        let c_i = ?a' [\<oplus>] p_i in
+        c_i # enc_loop_func_list (nat_to_bitstring h, n, h, c') x_i
+        ) = a # m" by auto
+  hence "enc_loop_func_list (nat_to_bitstring h, n, h, ?a' # c') x = a # m" by auto  
+  then show ?case using c_obtain by auto
 qed
-
-
-lemma "enc_loop (21, 2, [[True, False], [True, False], [True, False]]) 9 = 
-  ([[False, False], [True, True], [False, False]], 18)" 
-  apply (auto simp add: xor_list_def nat_to_bitstring_def nat_to_words_len_def)
-  by (auto simp add: nat_to_words_def)
 
 (* TODO: Clean everything out! E.g. put supporting auxiliary functions to BG_aux.thy.  *)
 (* TODO: Check if this works as intended! - But how? *)
